1. Absorption
	1. $x+x\cdot y=x$
		1. $\rightarrow (x+x)\cdot(x+y)$
		2. if $x=0:(0+0)\cdot(0+y)=0$
		3. if $x=1:(1+1)\cdot(1+y)=1$
	2. $x\cdot(x+y)=x$
		1. $\rightarrow(x\cdot x)+(x\cdot y)$
		2. if $x=0:(0\cdot0)+(0\cdot y)=0$
		3. if $x=1:(1\cdot1)+(1\cdot y)=1$
2. Combining
	1. $x\cdot y+x\cdot\overline{y}=x$
		1. if $x=0:(0\cdot y)+(0\cdot\overline{y})=0$
		2. if $x=1:(1\cdot y)+(1\cdot\overline{y})=1$
	2. $(x+y)\cdot(x+\overline{y})=x$
		1. if $x=0:(0+y)\cdot(0+\overline{y})=0$
		2. if $x=1:(1+y)\cdot(1+\overline{y})=1$
3. DeMorgan's Theorem
	1. $\overline{x\cdot y}=\overline{x}+\overline{y}$
	2. $\overline{x+y}=\overline{x}\cdot\overline{y}$
4. More Absorption
	1. $x+\overline{x}\cdot y=x+y$
		1. $\rightarrow (x+\overline{x})\cdot(x+y)$
		2. $\rightarrow 1\cdot(x+y)$
	2. $x\cdot(x+y)=x\cdot y$
		1. $\rightarrow (x\cdot x)+(x\cdot y)$
5. Consensus
	1. $x\cdot y+y\cdot z+ \overline{x}\cdot z = x\cdot y + \overline{x}\cdot z$
	2. $(x+y)\cdot(y+z)\cdot(\overline{x}+z)=(x+y)\cdot(\overline{x}+z)$